src/Impl_vm.v
@@ -33,7 +33,7 @@ Fixpoint copland_compile (t:AnnoTerm): CVM unit :=
   | alseq _ t1 t2 =>
       copland_compile t1 ;;
       copland_compile t2
- (* | abseq (x,y) _ (sp1,sp2) t1 t2 =>
+  | abseq (x,y) (sp1,sp2) t1 t2 =>
       e <- get_ev ;;
       p <- get_pl ;;
       pr <- split_ev_seq x sp1 sp2 e p ;;
@@ -45,6 +45,7 @@ Fixpoint copland_compile (t:AnnoTerm): CVM unit :=
       copland_compile t2 ;;
       e2r <- get_ev ;;
       join_seq (Nat.pred y) p e1r e2r
+               (*
   | abpar (x,y) _ (*(loc_e1,loc_e1')*) (loc_e2,loc_e2') (sp1,sp2) t1 t2 =>
       e <- get_ev ;;
       p <- get_pl ;;
